dev/make-all.sh
@@ -1,3 +1,5 @@
 #!/bin/bash
 
 lake update && lake build # && lake test
+
+if command -v markdownlint >/dev/null 2>&1; then markdownlint '**/*.md'; fi
